src/CSL/Counting.v
@@ -1,0 +1,85 @@
+From iris.algebra Require Import proofmode_classes.
+From iris.base_logic Require Import base_logic.
+Set Default Proof Using "Type".
+
+Inductive counting :=
+| Count (z: Z)
+| CountBot.
+
+Local Open Scope Z.
+
+Instance counting_valid : Valid counting := λ x,
+  match x with Count _ => True | CountBot => False end.
+Instance counting_validN : ValidN counting := λ n x,
+  match x with Count _ => True | CountBot => False end.
+Instance counting_pcore : PCore counting := λ x, None.
+Instance counting_op : Op counting :=
+  λ x y,
+  match x, y with
+  | Count z1, Count z2 =>
+    if (decide (z1 >= 0 ∧ z2 >= 0)) then CountBot else
+    if (decide ((z1 >= 0 ∨ z2 >= 0) ∧ (z1 + z2) < 0)) then CountBot else
+      Count (z1 + z2)
+  | _, _ => CountBot
+  end.
+Canonical Structure countingC := leibnizC counting.
+
+Local Ltac by_cases :=
+  repeat (match goal with
+          | [ H: counting |- _ ] => destruct H
+          | [ H: counting |- _ ] => destruct H
+          end) => //=;
+  repeat destruct decide => //=; try lia.
+
+Lemma counting_ra_mixin : RAMixin counting.
+Proof.
+  split; try apply _; try done.
+  - intros x y z. rewrite /op/counting_op.
+    by_cases. f_equal. lia.
+  - intros x y. rewrite /op/counting_op.
+    by_cases. f_equal. lia.
+  - intros x y. rewrite /op/counting_op/valid.
+    by_cases.
+Qed.
+
+Canonical Structure countingR := discreteR counting counting_ra_mixin.
+
+Global Instance counting_cmra_discrete : CmraDiscrete countingR.
+Proof. apply discrete_cmra_discrete. Qed.
+
+Lemma counting_op' (x y : countingR) : (x ⋅ y) = (counting_op x y).
+Proof. done. Qed.
+
+Lemma counting_valid' (x : countingR) : ✓ x ↔ (counting_valid x).
+Proof. done. Qed.
+
+Lemma counting_validN' n (x : countingR) : ✓{n} x ↔ (counting_validN n x).
+Proof. done. Qed.
+
+Global Instance is_op_counting z :
+  z >= 0 → IsOp' (Count z) (Count (z + 1)) (Count (-1)).
+Proof.
+  rewrite /IsOp' /IsOp counting_op' => ?.
+  rewrite //=. by_cases. f_equal. lia.
+Qed.
+
+Global Instance is_op_counting' (n: nat) :
+  IsOp' (Count n) (Count (S n)) (Count (-1)).
+Proof.
+  rewrite /IsOp' /IsOp counting_op' //=.
+  by_cases. f_equal. lia.
+Qed.
+
+Global Instance counting_id_free (z : counting) : IdFree z.
+Proof.
+  intros y.
+  rewrite counting_op' counting_validN'.
+  by_cases. destruct y; by_cases; intros _; inversion 1.
+  lia.
+Qed.
+
+Global Instance counting_full_exclusive : Exclusive (Count 0).
+Proof.
+  intros y. rewrite counting_validN' counting_op'.
+  destruct y => //=; by_cases. 
+Qed.
